Good progress on partial function application
Worked through the application case enough to be confident that the
evaluation order stuff works. Had to change the location of closure
arguments to functions in the code table to be the first argument rather
than the last (e.g., Var n for an n argument function, rather than Var 0
always). This is a bit more complicated, but the advantage is that App
(SOME l) x xs can be compiled to Call (SOME l) (xs++[x]), instead of
Let (xs++x) (Call (SOME l) [Var n; Var 0; ...; Var (n-1)] ). The App
NONE case requires a let since the closure must be evaluated last, and
only once.

new-backend/closLangScript.sml
@@ -292,8 +292,9 @@ val lookup_vars_def = Define `
      else NONE)`
 
 val check_loc_opt_def = Define `
-  (check_loc NONE loc num_params num_args ⇔ num_args < max_app) /\
-  (check_loc (SOME p) loc num_params num_args ⇔ (num_params = num_args) ∧ (p = loc))`;
+  (check_loc NONE loc num_params num_args so_far ⇔ num_args < max_app) /\
+  (check_loc (SOME p) loc num_params num_args so_far ⇔ 
+    (num_params = num_args + so_far) ∧ (p = loc))`;
 
 val _ = Datatype `
   app_kind =
@@ -304,8 +305,8 @@ val dest_closure_def = Define `
   dest_closure loc_opt f args =
     case f of
     | Closure loc arg_env clo_env num_args exp =>
-        if check_loc loc_opt loc num_args (LENGTH args) ∧ LENGTH arg_env < num_args then
-          if LENGTH args + LENGTH arg_env > num_args then
+        if check_loc loc_opt loc num_args (LENGTH args) (LENGTH arg_env) ∧ LENGTH arg_env < num_args then
+          if ¬(LENGTH args + LENGTH arg_env < num_args) then
             SOME (Full_app exp
                            (REVERSE (TAKE (num_args + 1 - LENGTH arg_env) (REVERSE args))++
                             arg_env++clo_env)
@@ -316,9 +317,11 @@ val dest_closure_def = Define `
           NONE
     | Recclosure loc arg_env clo_env fns i =>
         let (num_args,exp) = EL i fns in
-          if LENGTH fns <= i \/ ~(check_loc loc_opt (loc+i) num_args (LENGTH args)) ∨ ¬(LENGTH arg_env < num_args) then NONE else
+          if LENGTH fns <= i \/ 
+             ~(check_loc loc_opt (loc+i) num_args (LENGTH args) (LENGTH arg_env)) ∨
+             ¬(LENGTH arg_env < num_args) then NONE else
             let rs = GENLIST (Recclosure loc [] clo_env fns) (LENGTH fns) in
-              if LENGTH args + LENGTH arg_env > num_args then
+              if ¬(LENGTH args + LENGTH arg_env < num_args) then
                 SOME (Full_app exp
                                (REVERSE (TAKE (num_args + 1 - LENGTH arg_env) (REVERSE args))++
                                 arg_env++rs++clo_env)
@@ -328,7 +331,7 @@ val dest_closure_def = Define `
     | _ => NONE`;
 
 val dest_closure_length = Q.prove (
-`!loc_opt f args exp args1 args2.
+`!loc_opt f args exp args1 args2 so_far.
   dest_closure loc_opt f args = SOME (Full_app exp args1 args2)
   ⇒
   LENGTH args2 < LENGTH args`,
@@ -339,7 +342,7 @@ val dest_closure_length = Q.prove (
  TRY decide_tac >>
  Cases_on `EL n l1` >>
  fs [LET_THM] >>
- Cases_on `LENGTH args + LENGTH l > q` >>
+ Cases_on `LENGTH args + LENGTH l < q` >>
  fs [] >>
  rw [] >>
  decide_tac);
